SEARsettings.sml
@@ -1,3 +1,34 @@
+fun fVar_Inst1 (pair as (P,(argl:(string * sort) list,Q))) f = 
+    case view_form f of
+        vfVar(P0,args0) =>
+(*ListPair.map ListPair.foldl*)
+(*mk_inst (zip argl args0)ListPair. [] *)
+        if P0 = P then
+            let val venv = match_tl essps (List.map mk_var argl) args0 emptyvd 
+            in inst_form (mk_menv venv emptyfvd) Q
+            end
+(*if the number of arguments is wrong, or the sorts is wrong, then handle the matching exn by returning f *)
+        else f
+      | vConn(co,fl) => mk_conn co (List.map (fVar_Inst1 pair) fl)
+      | vQ(q,n,s,b) => mk_quant q n s (fVar_Inst1 pair b)
+      | vPred _ => f
+
+(*ex2fsym should check that the input thm does not contain fvars*)
+
+fun fVar_Instl l f = 
+    case l of [] => f
+            | pair :: t => fVar_Inst1 pair (fVar_Instl t f)
+
+fun fVar_Inst l th = 
+    let val (ct,asl,w) = dest_thm th
+        val asl' = List.map (fVar_Instl l) asl
+        val w' = fVar_Instl l w
+        val vs = bigunion (pair_compare String.compare sort_compare)
+                          (List.map fvf (w' :: asl'))
+        val newct = HOLset.union(ct,vs)
+    in mk_thm (newct,asl',w')
+    end
+
 
 local
 fun delete'(set,mem) = HOLset.delete(set,mem) handle _ => set
@@ -69,99 +100,6 @@ fun dest_mem_sort s =
 *)
 
 
- fVarInst : (string * (var list * form)) list -> thm -> thm
-
-entry point.  The variables are the bound variables and the form is the body of the abstraction.  Then after you substitute, you check that the list of arguments is the right length, and then do the beta-reduction to eliminate the bound variables.
-
-fun abstractl l fm = 
-    case l of [] => fm
-            | h :: t => abstract h (abstractl t fm)
- 
-fun fVarInst_fm1 (pair as (fvn:string,(vl:(string * sort) list,fm:form))) f0 = 
-    case view_form f0 of 
-        vfVar(fv0,args) => 
-        if fv0 = fvn then if length args = length vl then
-                             (* abstractl vl *) fm
-                          else raise ERR ("fVarInst.list length differs.",[],[],[f0])
-        else f0
-      | vQ(q,n,s,b) => mk_quant q n s (fVarInst_fm1 pair b)
-      | vConn(co,l) => mk_conn co (List.map (fVarInst_fm1 pair) l)
-      | vPred _ => f0
-
-fun subst_form (f0,f) fm = 
-    case view_form fm of 
-
-val ifffm = “!a b. P(a,b) <=> Holds(Q:B->A,b,a)”
-fun fVarInst_fm1 ifffm f0 = 
-    let val (iff,bvs) = strip_forall ifffm 
-        val (fV,actu) = dest_dimp iff 
-
-
-
-(*
-
-fun fVarInst_fm1 Q l ct f0 = 
-    let val Qfvs = fvf Q
-        val (orgvs,tms) = List.map fst l
-        (*variables in Q to terms which can be constructed from ct*)
-        val _ = HOLset.isSubset(List.foldr (fn (t,set) => HOLset.union(fvt t,set)) essps tms,ct) orelse
-                raise ERR ("fVarInst_fm1, extra variables.",[],[],[f0])
-        val Q' = mk_inst l [] Q
-        val _ = HOLset.isSubset(fvf Q',ct)
-        val 
-*)
-fun fVarInst_fm pairl f0 = 
-List.foldr (uncurry fVarInst_fm1) f0 pairl
-
-val AX1 = new_ax
-“!A B:set.?!R:A->B.!a:mem(A) b:mem(B).Holds(R,a,b)<=> P(a,b)”
-
-
-val f0 = concl AX1
-val fm = “Holds(Q:B->A,b,a)”
-val fvn = "P"
-val vl = [("a",mem_sort (mk_set "A")),("b",mem_sort (mk_set "B"))]
-val pair = (fvn,(vl,fm))
-
-fVarInst_fm1 pair f0
-
-want inst 
-fVarInst_fm1 pair $ concl AX1
-val f0 = “!b:mem(C). Q(b) & (!b:mem(B).Holds(R:A->B,a,b) <=>P(a,b))”
-
-
-
-val f0 = “!b:mem(B).P(a,b)”
-
-val f0 = “P(a:mem(A),b:mem(B))”
-fun fVarInst_fm l f = 
-    case l of 
-        [] => f
-      | (fvn,(vl,fm)) :: t => 
-        let val f' = fVarInst_fm t f
-            val 
-fun fVarInst l th = 
-    case l of 
-        [] => th 
-      | h :: t =>
-        let val (ct,asl,w) = dest_thm th
-            val 
-
-
-(*
-inst_thm (mk_inst 
-              [(("a",mem_sort $mk_set "A"),mk_var("a",mem_sort $mk_set "A")),
-               (("b",mem_sort $mk_set "B"),mk_var("b",mem_sort $mk_set "B"))] [("P",“Holds(Q:A->B,a,b)”)]) (spec_all AX1)
-*)
-
-
-(*must be able to inst the P(a,b) into P0(B(1),B(0))
-in the case that 
-
-*)
-
-
-
 fun AX1 (f:form) (a0 as (n1,s1),b0 as (n2,s2)) = 
     let val fvs = fvf f
         val a = mk_var a0
@@ -193,17 +131,14 @@ val _ = new_pred "isBij" [("R",rel_sort (mk_set "A") (mk_set "B"))]
 val Fun_def = new_ax “!A B R:rel(A,B). isFun(R) <=> !x:mem(A). ?!y:mem(B). Holds(R,x,y)”
 
 
-(*
-val _ = rapf "!A B R:rel(A,B). isFun(R) <=> !x:mem(A). ?!y:mem(B). Holds(R,x,y)";
-*)
-
 val _ = new_fun "Eval" (mem_sort (mk_set "B"),[("R",rel_sort (mk_set "A") (mk_set "B")),
                         ("x",mem_sort (mk_set "A"))]) 
 
 val Eval_def = new_ax “!A B Fn:rel(A,B). isFun(Fn) ==>!x y. Holds(Fn,x,y) <=> y = Eval(Fn,x)”
 
-val Inj_def = new_ax “!A B R:rel(A,B). isInj(R) <=> !x1:mem(A) x2:mem(A) y:mem(B). Holds(R,x1,y) & Holds(R,x2,y) ==> x1 = x2”
-val Surj_def = new_ax “!A B R:rel(A,B). isSurj(R) <=> !y:mem(B).?x:mem(A). Holds(R,x,y)”
+val Inj_def = new_ax “!A B R:rel(A,B). isInj(R) <=> isFun(R) & !x1:mem(A) x2:mem(A). Eval(R,x1) = Eval(R,x2) ==> x1 = x2”;
+val Surj_def = new_ax “!A B R:rel(A,B). isSurj(R) <=> isFun(R) & !y:mem(B).?x:mem(A). Eval(R,x) = y”;
+val Bij_def = new_ax “!A B R:A->B. isBij(R) <=> isInj(R) & isSurj(R)”;
 
 val _ = new_pred "isTab" [("R",rel_sort (mk_set "A") (mk_set "B")),
                           ("p",rel_sort (mk_set "TR") (mk_set "A")),
@@ -211,7 +146,7 @@ val _ = new_pred "isTab" [("R",rel_sort (mk_set "A") (mk_set "B")),
 
 val Tab_def = new_ax
 “!A B R TR p:TR->A q:TR->B.isTab(R,p,q) <=> 
- (!x y. Holds(R,x,y) <=> ?r. Eval(p,r) = x & Eval(q,r) = y) & !r s. Eval(p,r) = Eval(p,s) & Eval(q,r) = Eval(q,s) ==> r = s”
+ isFun(p) & isFun(q) & (!x y. Holds(R,x,y) <=> ?r. Eval(p,r) = x & Eval(q,r) = y) & !r s. Eval(p,r) = Eval(p,s) & Eval(q,r) = Eval(q,s) ==> r = s”
 
 (*
 Axiom 2 (Tabulations): For any relation φ:A↬B, there exists a set |φ| and functions p:|φ|→A and q:|φ|→B such that: (1) for any x∈A and y∈B, we have φ(x,y) if and only if there exists r∈|φ| with p(r)=x and q(r)=y, and (2) for any r∈|φ| and s∈|φ|, if p(r)=p(s) and q(r)=q(s), then r=s.
@@ -225,7 +160,8 @@ val _ = new_fun "π2" (rel_sort (mk_set "TR") (mk_set "B"),[("R",rel_sort (mk_se
 *)
 
 (*how to let the ex2fsym function skip the TR and assign function symbols pi1 pi2?*)
-val AX2 = new_ax “!A B R:A->B.?TR p:TR->A q:TR->B. (!x y. Holds(R,x,y) <=> ?r. Eval(p,r) = x & Eval(q,r) = y) & !r s. Eval(p,r) = Eval(p,s) & Eval(q,r) = Eval(q,s) ==> r = s”
+
+val AX2 = new_ax “!A B R:A->B.?TR p:TR->A q:TR->B. isFun(p) & isFun(q) & (!x y. Holds(R,x,y) <=> ?r. Eval(p,r) = x & Eval(q,r) = y) & !r s. Eval(p,r) = Eval(p,s) & Eval(q,r) = Eval(q,s) ==> r = s”
 
 (*
 Theorem 2.2. There exists a set ∅ which has no elements.
@@ -236,6 +172,37 @@ Proof. By Axiom 0, there exists a set A. By Axiom 1, there exists a relation φ:
 (*how can we just type the name once? for prove_store*)
 (*rw you idiot gives me  ~(~a'' = a'' & b = b)*)
 
+
+val AX1 = new_ax
+“!A B:set.?!R:A->B.!a:mem(A) b:mem(B).Holds(R,a,b)<=> P(a,b)”
+
+(*
+val f0 = concl AX1
+val fm = “Holds(Q:B->A,b,a)”
+val fvn = "P"
+val vl = [("a",mem_sort (mk_set "A")),("b",mem_sort (mk_set "B"))]
+val pair = (fvn,(vl,fm))
+
+val _ = fVar_Inst1 pair f0
+*)
+
+val lemma = fVar_Inst [("P",([("a",mem_sort (mk_set "A")),("b",mem_sort (mk_set "A"))],“~(a:mem(A) = a)”))] (AX1 |> qspecl [‘A’,‘A’])
+val lemma' = dimp_mp_l2r lemma (uex_def $ concl lemma) 
+val Thm_2_2 = proved_th $ (*val (ct,asl,w) = cg $*)
+e0
+(strip_assume_tac AX0 >> strip_assume_tac lemma' >>
+ qspecl_then [‘A’,‘A’,‘R’] strip_assume_tac AX2 >>
+ qexists_tac ‘TR’ >> strip_tac >> 
+ by_tac “!a b. ~Holds(R:A->A,a:mem(A),b:mem(A))” 
+ >-- (rpt strip_tac >> pop_assum (K all_tac) >> pop_assum (K all_tac) >>
+      once_arw[] >> ccontra_tac >> fs[]) >>
+ suffices_tac “Holds(R:A->A,Eval(p:TR->A,a'),Eval(q:TR->A,a':mem(TR)))”
+ >-- arw[] >>
+ pop_assum (K all_tac) >> arw[] >> qexists_tac ‘a'’ >> rw[])
+(form_goal
+“?Empty. !a:mem(Empty).F”)
+
+(*
 local
 val lemma = AX1 “~(a:mem(A) = a) & b:mem(A) = b” (("a",mem_sort (mk_set "A")),("b",mem_sort (mk_set "A")))
 val lemma' = dimp_mp_l2r lemma (uex_def $ concl lemma) 
@@ -254,24 +221,34 @@ e0
 (form_goal
 “?Empty. !a:mem(Empty).F”)
 end
-
-
-(*
- val (ct,asl,w) = cg $
-e0
-(strip_assume_tac AX0 >> strip_assume_tac lemma' >>
- qspecl_then [‘A’,‘A’,‘R’] strip_assume_tac AX2 >>
- qexists_tac ‘TR’ >> strip_tac >> 
- by_tac “!a b. ~Holds(R:A->A,a:mem(A),b:mem(A))” 
- >-- (rpt strip_tac >> pop_assum (K all_tac) >> pop_assum (K all_tac) >>
-      pop_assum (K all_tac) >> last_x_assum (K all_tac) >> once_arw[] >> rw[]))
-(form_goal
-“?Empty. !a:mem(Empty).F”)
 *)
+
 
 
 val _ = store_thm("Thm_2_2",Thm_2_2)
 
+val lemma = fVar_Inst [("P",([("y",mem_sort (mk_set "A")),("z",mem_sort (mk_set "A"))],“y = a0:mem(A) & z = a0”))] (AX1 |> qspecl [‘A’,‘A’])
+val lemma' = dimp_mp_l2r lemma (uex_def $ concl lemma)
+
+
+val Thm_2_3 = proved_th $ 
+e0
+(x_choosel_then ["A","a0"] assume_tac AX0 >> 
+ strip_assume_tac lemma' >>
+ qspecl_then [‘A’,‘A’,‘R’] strip_assume_tac AX2 >>
+ qby_tac ‘Holds(R,a0,a0)’ >--
+ (pop_assum (K all_tac) >> pop_assum (K all_tac) >> arw[]) >>
+ pop_assum mp_tac >> once_arw[] >> strip_tac  >>
+ qexistsl_tac [‘TR’,‘r’] >> 
+ strip_tac >> first_x_assum irule >> arw[] >>
+ fs[] >>
+ once_rw[CONJ_COMM] >> first_x_assum $ (irule o iffLR) >>
+ qexists_tac ‘x'’ >> rw[])
+(form_goal
+“?ONE x:mem(ONE). !x':mem(ONE). x' = x”)
+
+
+(*
 local 
 val lemma = AX1 “y = a:mem(A) & z = a” (("y",mem_sort (mk_set "A")),("z",mem_sort (mk_set "A")))
 val lemma' = dimp_mp_l2r lemma (uex_def $ concl lemma) 
@@ -292,30 +269,31 @@ e0
 (form_goal
 “?ONE x:mem(ONE). !x':mem(ONE). x' = x”)
 end
+*)
 
 
+val ONE_def = Thm_2_3 |> eqT_intro |> iffRL |> ex2fsym "1" []
+                      |> C mp (trueI []) |> gen_all
+val dot_def = ONE_def |> eqT_intro |> iffRL |> ex2fsym "dot" []
+                      |> C mp (trueI []) |> gen_all
 
-val _ = new_fun "1" (set_sort,[])
 val ONE = mk_fun "1" []
-val _ = new_fun "star" (mem_sort ONE,[])
 
-
-
+val dot = mk_fun "dot" []
+(*
 fun Rel2Pred P (ns as (n,s)) =
     let val onens = ("one0",mem_sort ONE)
         val conj1 = mk_eq (mk_var onens) (mk_var onens)
     in AX1 (mk_conj conj1 P)  (onens,ns)
     end
-
-val Thm_2_4_R_ver = proved_th $
-e0
-(cheat)
-(form_goal
-“!A R:1 -> A. ?B i:B->A. !a:mem(A).Holds(R,star,a) <=> ?b. a = Eval(i,b)”)
-
-(*
-Theorem 2.4. For any property P of elements of a set A, there exists a set B and an injective function i:B→A such that for a∈A, we have P(a) iff a=i(b) for some b∈B.
 *)
+val R_EXT = new_ax “!A B R1:A->B R2. R1 = R2 <=> !a b.Holds(R1,a,b) <=> Holds(R2,a,b)”
+
+val FUN_EXT = proved_th $
+e0
+cheat
+(form_goal “!A B f1:A->B f2. isFun(f1) & isFun(f2) ==>
+ (f1 = f2 <=> (!a.Eval(f1,a) = Eval(f2,a)))”)
 
 fun uex_ex f = 
     let val th0 = iffLR $ uex_def f |> undisch
@@ -326,6 +304,143 @@ fun uex_ex f =
         val th3 = existsE (n,s) th0 th2
     in disch f th3
     end
+
+fun uex2ex_rule th = mp (uex_ex $concl th) th
+fun uex_expand th = rewr_rule [uex_def $ concl th] th
+
+
+(*TODO; make !a.T. in rw*)
+(*TODO: tactic for expand uex in goal*)
+local 
+val lemma = 
+(fVar_Inst [("P",([("a",mem_sort (mk_set "A")),("b",mem_sort ONE)],“a = a:mem(A)”))] (AX1 |> qspecl [‘A’,‘1’])) 
+val lemma' = uex_expand lemma
+in
+val Thm_2_3_5 = proved_th $
+e0
+(strip_tac >> rw[uex_def “?!f:A->1.isFun(f)”,R_EXT] >> 
+ strip_assume_tac lemma' >> qexists_tac ‘R’ >> rw[Fun_def] >> strip_tac (* 2 *)
+ >-- (strip_tac >> rw[uex_def “?!y:mem(1).Holds(R,x,y)”] >>
+      qexists_tac ‘dot’ >> once_rw[dot_def] >>
+      arw[] >> strip_tac >> rw[]) >>
+ strip_tac >> strip_tac >> rw[GSYM R_EXT] >> first_x_assum irule >>
+ strip_tac >> first_x_assum (qspecl_then [‘a’] assume_tac) >>
+ pop_assum (strip_assume_tac o uex_expand) >>
+ pop_assum (K all_tac) >> pop_assum mp_tac >> once_rw[dot_def] >>
+ rpt strip_tac >> arw[])
+(form_goal
+“!A.?!f:A->1. isFun(f)”)
+end
+
+val Thm_2_3_5_expand = Thm_2_3_5 |> spec_all |> uex_expand |> gen_all
+
+val To1_def = Thm_2_3_5_expand |> spec_all |> eqT_intro |> iffRL |> ex2fsym "To1" ["A"]
+                        |> C mp (trueI []) |> gen_all
+
+
+val Thm_2_4_R_ver = proved_th $
+e0
+(rpt strip_tac >> qspecl_then [‘1’,‘A’,‘R’] strip_assume_tac AX2 >>
+ qexistsl_tac [‘TR’,‘q’] >>
+ once_arw[] >> strip_tac (* 2 *)
+ >-- (rw[Inj_def] >> arw[] >> rpt strip_tac >> first_x_assum irule >>
+      arw[] >> once_rw[dot_def] >> rw[] (*Eval(p, x1) = Eval(p, x2) as 1 is tml*)) >>
+ strip_tac >> dimp_tac >> rpt strip_tac (* 2 *)
+ >-- (qexists_tac ‘r’ >> arw[]) >>
+ qexists_tac ‘b’ >> arw[] >> once_rw[dot_def] >> rw[])
+(form_goal
+“!A R:1 -> A.?B i:B->A. isInj(i) & !a:mem(A).Holds(R,dot,a) <=> ?b. a = Eval(i,b)”)
+
+(*“?a0:mem(A) ==> (!a:mem(A).P(b)) <=> P(b)” 
+think about if this can be proved and behave in the desired way.
+
+*)
+
+local
+val l0 = (fVar_Inst [("P",([("a",mem_sort ONE),("b",mem_sort (mk_set "A"))],“a = a:mem(1) & P(b:mem(A))”))] (AX1 |> qspecl [‘1’,‘A’])) |> gen_all
+val uth = uex_def “?!R:1->A. !a. Holds(R, dot, a) <=> P(a)”
+in
+val Rel_Pred1 = proved_th $
+e0
+(assume_tac l0 >> strip_tac >>
+ first_x_assum (qspecl_then [‘A’] assume_tac) >>
+ first_assum (fn th => assume_tac (uex_def $ concl th)) >> fs[] >>
+ rw[uth] >> qexists_tac ‘R’ >> once_arw[] >> rw[] >> conj_tac (* 2 *)
+ >-- (strip_tac >> once_rw[]) >> 
+ rpt strip_tac >> first_x_assum irule >> once_rw[dot_def] >> arw[] >>
+ rpt strip_tac >> rw[])
+(form_goal
+“!A. ?!R:1->A.!a:mem(A). Holds(R,dot,a) <=> P(a)”)
+end
+
+(*TODO: fs[] with
+ a
+   1.!(a : set). P(a#) <=> Q(a#)
+   2.!(a : set). P(a#)
+   ----------------------------------------------------------------------
+   Q(a)
+
+loops
+
+rfs[] loops as well, and if cut, then err is:
+ ERR
+     ("mp.no match", [], [],
+      [Conn ("==>", [Pred ("T", []), fVar ("P", [a])]), fVar ("Q", [a])])
+   raised
+*)
+
+val rfs =  rev_full_simp_tac;
+
+(*
+val Pred_Rel1 =
+“!A. ?!R:1->A.!a:mem(A). P(a) <=> Holds(R,dot,a)”)
+*)
+
+
+(*
+val lemma = fVar_Inst [("P",([("y",mem_sort (mk_set "A")),("z",mem_sort (mk_set "A"))],“y = a0:mem(A) & z = a0”))] (AX1 |> qspecl [‘1’,‘A’])
+val lemma' = dimp_mp_l2r lemma (uex_def $ concl lemma)
+*)
+
+val th= assume “Holds(R:1->A,dot,a) <=> P(a)”
+
+val f = “Holds(R:1->A,dot,a) <=> Holds(Q,a,b)”
+basic_fconv no_conv (rewr_fconv th) f
+(*
+
+ BA(i : rel(B, A))(R : rel(1, A))
+   1.!(A : set).
+               ?!(R : rel(1, A#)).
+                 !(a : mem(A#)). Holds(R#, dot, a#) <=> P(a#)
+   2.!(a : mem(A)). Holds(R, dot, a#) <=> P(a#)
+   3.isInj(i)
+   4.!(a : mem(A)). Holds(R, dot, a#) <=> ?(b : mem(B)). a# = Eval(i, b#)
+   ----------------------------------------------------------------------
+   T & !(a : mem(A)). P(a#) <=> ?(b : mem(B)). a# = Eval(i, b#)
+
+rfs loops
+*)
+
+
+local
+val lemma = mp (uex_ex (concl $ spec_all Rel_Pred1)) (spec_all Rel_Pred1) 
+in
+val Thm_2_4 = proved_th $
+e0
+(assume_tac Thm_2_4_R_ver >> strip_tac >>
+ strip_assume_tac lemma >>
+ first_x_assum (qspecl_then [‘A’,‘R’] strip_assume_tac) >>
+ qexistsl_tac [‘B’,‘i’] >> once_arw[] >> pop_assum (assume_tac o GSYM) >>
+ (*if instead of GSYM above use fs then loop*)
+ rw[] >> strip_tac >> once_arw[] >> once_arw[] >> rw[]
+ )
+(form_goal
+“!A.?B i:B->A. isInj(i) & !a:mem(A).P(a) <=> ?b. a = Eval(i,b)”)
+end
+
+(*
+Theorem 2.4. For any property P of elements of a set A, there exists a set B and an injective function i:B→A such that for a∈A, we have P(a) iff a=i(b) for some b∈B.
+*)
 
 (*val P = “a:mem(A) = b”*)
 (*P(a#)
@@ -353,6 +468,8 @@ P(f(a))
 
 a 
 *)
+
+(*
 val ns = ("a",mem_sort  (mk_set "A"))
 fun Thm_2_4 P (ns as (n,s)) = 
     let val l1 = Rel2Pred P ns
@@ -368,17 +485,113 @@ fun Thm_2_4 P (ns as (n,s)) =
         val exEed = existsE (r,rsort) l1'_cj2 insted'
     in exEed
     end
+*)
+
 
 (*
 Theorem 2.5. If |φ| and |φ|′ are two tabulations of the same relation φ:A↬B, then there is a bijection between |φ| and |φ|′.
 *)
 
+val Tab_Fun = proved_th $
+e0
+(rpt strip_tac >> fs[Tab_def])
+(form_goal
+“!A B R:A->B TR p:TR->A q:TR->B.isTab(R,p,q) ==>
+ isFun(p) & isFun(q)”)
+
+val Tab_Eval_Rel = proved_th $
+e0
+(rpt strip_tac >> fs[Tab_def] >>
+ qexists_tac ‘r’ >> arw[]
+ )
+(form_goal
+“!A B R:A->B TR p:TR->A q:TR->B.isTab(R,p,q) ==>
+ (!r x y. Eval(p,r) = x & Eval(q,r) = y ==> Holds(R,x,y))”)
+
+
+
+
+val Tab_mem_R = proved_th $
+e0
+(rpt strip_tac >> fs[Tab_def] >>
+ qexists_tac ‘r’ >> rw[])
+(form_goal
+ “!A B R:A->B TR p q. isTab(R,p:TR->A,q) ==> !r:mem(TR). Holds(R,Eval(p,r),Eval(q,r))”)
+
+val Tab_prop1 = proved_th $
+e0
+(rpt strip_tac >> fs[Tab_def])
+(form_goal 
+“!A B R:A->B TR p:TR->A q:TR->B.
+ isTab(R,p,q) ==> 
+ (!x y. Holds(R,x,y) <=> ?r:mem(TR).Eval(p,r) = x & Eval(q,r) = y)”)
+
+
+val Tab_prop2 = proved_th $
+e0
+(rpt strip_tac >> fs[Tab_def] >> first_x_assum irule >> arw[])
+(form_goal 
+“!A B R:A->B TR p:TR->A q:TR->B.
+ isTab(R,p,q) ==> 
+ (!r s. Eval(p,r) = Eval(p,s) & Eval(q,r) = Eval(q,s) ==> r = s)”)
+
+
+(*TODO:
+!(x : mem(T1))  (y : mem(T2)). y# = Eval(B0, x#) <=> Holds(B0, x#, y#)
+
+flip = in this
+
+*)
+
+fun eq_sym a = 
+    if mem a (!EqSorts) then 
+        let val ns0 = srt2ns a
+            val v1 = mk_var ns0
+            val v2 = pvariantt (HOLset.add(essps,ns0)) v1
+            val v1v2 = mk_eq v1 v2
+            val v2v1 = mk_eq v2 v1
+            val l2r = assume v1v2 |> sym|> disch_all
+            val r2l = assume v2v1 |> sym|> disch_all
+        in dimpI l2r r2l
+        end
+    else raise ERR ("eq_sym.input sort: " ^ a ^ " does not have equality",
+                    [],[],[])
+
+
+local
+val lemma = fVar_Inst [("P",([("a",mem_sort (mk_set "T1")),("b",mem_sort (mk_set "T2"))],“Eval(p1:T1->A,a) = Eval(p2:T2->A,b) & Eval(q1:T1->B,a) = Eval(q2:T2->B,b)”))] (AX1 |> qspecl [‘T1’,‘T2’])
+val lemma' = dimp_mp_l2r lemma (uex_def $ concl lemma) 
+in
 val Thm_2_5 = proved_th $
 e0
-(cheat)
+(rpt strip_tac >> x_choose_then "B0" strip_assume_tac lemma' >> 
+ qexists_tac ‘B0’ >> rw[Bij_def] >> 
+ qby_tac ‘isFun(B0)’ >--
+ (rw[Fun_def] >> strip_tac >>
+  rw[uex_def “?!y:mem(T2).Holds(B0:T1->T2,x,y)”] >>
+  arw[] >> rev_drule Tab_mem_R >> 
+  first_x_assum (qspecl_then [‘x’] assume_tac) >>
+  drule Tab_prop1 >> fs[] >>
+  qexists_tac ‘r’ >> arw[] >> drule Tab_prop2 >>
+  rpt strip_tac >> first_x_assum irule >> arw[]) >>
+ rw[Inj_def,Surj_def] >> arw[] >> strip_tac (* 2 *)
+ >-- (rev_drule Tab_prop2 >> rpt strip_tac >> first_x_assum irule >>
+      drule Eval_def >>
+      first_assum (qspecl_then [‘x1’,‘Eval(B0,x1)’] assume_tac) >>
+      first_x_assum (qspecl_then [‘x2’,‘Eval(B0,x2)’] assume_tac) >>
+      first_assum (qspecl_then [‘x1’,‘Eval(B0,x1)’] assume_tac) >>
+      first_assum (qspecl_then [‘x2’,‘Eval(B0,x2)’] assume_tac) >> 
+      fs[]) >>
+ (*Surj*)
+ strip_tac >>
+ fconv_tac (once_depth_fconv no_conv (rewr_fconv (eq_sym "mem"))) >>
+ drule $ GSYM Eval_def >> arw[] >>
+ drule Tab_mem_R >> first_x_assum (qspecl_then [‘y’] assume_tac) >>
+ rev_drule Tab_prop1 >> fs[] >>
+ qexists_tac ‘r’ >> arw[])
 (form_goal
 “!A B R:A->B T1 p1:T1->A q1:T1->B T2 p2:T2->A q2:T2->B.isTab(R,p1,q1) & isTab(R,p2,q2) ==> ?b:T1 ->T2.isBij(b)”)
-
+end
 
 (*
 Corollary 2.6. If |S| and |S|′ are two tabulations of the same subset S⊆A, then there is a bijection between |S| and |S|′.
@@ -401,23 +614,195 @@ val o_def = new_ax
 val _ = new_fun "id" (rel_sort (mk_set "A") (mk_set "A"),
                      [("A",set_sort)])
 
+val id_def = new_ax “!A a:mem(A) b. Holds(id(A),a,b) <=> a = b”;
 
 val Thm_2_7_assoc = proved_th $
 e0
-(cheat)
+(rpt strip_tac >> rw[R_EXT,GSYM o_def] >> rpt strip_tac >>
+ dimp_tac >> rpt strip_tac (* 2 *)
+ >-- (qexists_tac ‘b''’ >> arw[] >> qexists_tac ‘b'’ >> arw[]) >>
+ qexists_tac ‘b''’ >> arw[] >> qexists_tac ‘b'’ >> arw[])
 (form_goal
 “!A B phi:A->B C psi:B->C D chi:C->D. (chi o psi) o phi = chi o psi o phi”)
 
+(*TODO:
+ ?(b' : mem(C)).
+               (?(b : mem(B)). Holds(phi, a, b#) & Holds(psi, b#, b'#)) &
+               Holds(chi, b'#, b)
+
+this should be simplified by using formula contains formula variables
+*)
 
 val Thm_2_7_id = proved_th $
 e0
-(cheat)
+(rpt strip_tac >> rw[R_EXT] >> rpt strip_tac  (* 2 *)
+ >-- (rw[GSYM o_def,id_def] >> dimp_tac >> rpt strip_tac
+      >-- arw[] >> qexists_tac ‘a’ >> arw[]) >>
+ rw[GSYM o_def,id_def] >> dimp_tac >> rpt strip_tac 
+ >-- fs[] >> qexists_tac ‘b’ >> arw[])
 (form_goal
 “!A B phi:A->B. phi o id(A) = phi & id(B) o phi = phi”)
 
+val _ = new_fun "op" (rel_sort (mk_set "B") (mk_set "A"),[("R",rel_sort (mk_set "A") (mk_set "B"))])
+
+val op_def = new_ax “!A B R:A->B a b.Holds(op(R),a,b) <=> Holds(R,b,a)”;
+
+
+(*
+
+todo
+val Bij_R = proved_th $
+e0
+()
+(form_goal
+ “!A B R:A->B.isBij(R) <=> 
+  !a.?!b.Holds(R,a,b) & !b.?!a.Holds(R,a,b)”)
+*)
+
+val Fun_expand = proved_th $
+e0
+(rpt strip_tac >> rw[Fun_def] >>
+ rw[uex_def “?!y:mem(B).Holds(R,x,y)”] >> 
+ dimp_tac >> strip_tac (* 2 *)
+ >-- (rpt strip_tac (* 2 *)
+     >-- (first_x_assum (qspecl_then [‘a’] assume_tac) >> 
+          pop_assum strip_assume_tac >> qexists_tac ‘y’ >> arw[]) 
+     >-- (first_x_assum (qspecl_then [‘a’] strip_assume_tac) >>
+          first_assum rev_drule >>
+          first_assum (qspecl_then [‘b2’] assume_tac) >>
+          first_assum drule >> arw[])) >>
+ rpt strip_tac >> last_x_assum (qspecl_then [‘x’] strip_assume_tac) >>
+ qexists_tac ‘b’ >> arw[] >> rpt strip_tac >> first_x_assum irule >>
+ qexists_tac ‘x’ >> arw[])
+(form_goal
+“!A B R:A->B. isFun(R) <=>
+ (!a.?b.Holds(R,a,b)) & 
+ (!a b1 b2. Holds(R,a,b1) & Holds(R,a,b2) ==> b1 = b2)”)
+
+val Inj_R_expand = proved_th $
+e0
+(rpt strip_tac >> rw[Inj_def,Fun_expand] >> dimp_tac >> strip_tac (* 2 *)
+ >-- (arw[] >> rpt strip_tac (* 3  2T*) >-- rw[] >-- rw[] >>
+      first_x_assum irule >> 
+      qby_tac ‘isFun(R)’ 
+      >-- (rw[Fun_expand] >> arw[] >> rpt strip_tac >-- rw[] >> rw[]) >>
+      drule Eval_def >> fs[]) >>
+ arw[] >> rpt strip_tac (* 3  2 T*) >-- rw[] >-- rw[] >>
+ first_x_assum irule >> qexists_tac ‘Eval(R,x1)’ >> 
+ qby_tac ‘isFun(R)’ 
+      >-- (rw[Fun_expand] >> arw[] >> rpt strip_tac >-- rw[] >> rw[]) >>
+ drule Eval_def >> arw[])
+(form_goal
+“!A B R:A->B. isInj(R) <=>
+ (!a.?b.Holds(R,a,b)) & 
+ (!a b1 b2. Holds(R,a,b1) & Holds(R,a,b2)==> b1 = b2) &
+ (!a1 a2 b. Holds(R,a1,b) & Holds(R,a2,b) ==> a1 = a2)”)
+
+val Surj_R_expand = proved_th $
+e0
+(rpt strip_tac >> rw[Surj_def,Fun_expand] >> dimp_tac >> strip_tac (* 2 *)
+ >-- (arw[] >> rpt strip_tac >-- rw[] >-- rw[] >>
+      qby_tac ‘isFun(R)’ 
+      >-- (rw[Fun_expand] >> arw[] >> rpt strip_tac >-- rw[] >> rw[]) >>
+      drule Eval_def >> arw[] >> 
+      fconv_tac (once_depth_fconv no_conv (rewr_fconv (eq_sym "mem"))) >>
+      arw[]) >>
+ arw[] >>
+ qby_tac ‘isFun(R)’ 
+ >-- (rw[Fun_expand] >> arw[] >> rpt strip_tac >-- rw[] >> rw[]) >>
+ rpt strip_tac >-- rw[] >-- rw[] >>
+ drule Eval_def >> fs[] >> 
+ fconv_tac (once_depth_fconv no_conv (rewr_fconv (eq_sym "mem"))) >>
+ arw[])
+(form_goal
+ “!A B R:A->B. isSurj(R) <=>
+ (!a.?b.Holds(R,a,b)) & 
+ (!a b1 b2. Holds(R,a,b1) & Holds(R,a,b2)==> b1 = b2) &
+ (!b. ?a.Holds(R,a,b))”)
+
+val Bij_R_expand = proved_th $
+e0
+(rpt strip_tac >> rw[Bij_def,Inj_R_expand,Surj_R_expand] >>
+ rpt strip_tac >> dimp_tac >-- (rpt strip_tac >>
+ arw[]
+ >-- (first_x_assum irule >> qexists_tac ‘a’ >> arw[]) >>
+ first_x_assum irule >> qexists_tac ‘b’ >> arw[]) >>
+ rpt strip_tac >> arw[] (* 3 *)
+ >-- (first_x_assum irule >> qexists_tac ‘a’ >> arw[])
+ >-- (first_x_assum irule >> arw[] >> qexists_tac ‘b’ >> arw[]) >>
+ first_x_assum irule >>
+ qexists_tac ‘a’ >> arw[])
+(form_goal
+ “!A B R:A->B. isBij(R) <=>
+ (!a.?b.Holds(R,a,b)) & 
+ (!a b1 b2. Holds(R,a,b1) & Holds(R,a,b2)==> b1 = b2) &
+ (!a1 a2 b. Holds(R,a1,b) & Holds(R,a2,b) ==> a1 = a2) &
+ (!b. ?a.Holds(R,a,b)) ”)
+
+
+
+
+
+(*
+
+qby_tac ‘!a. ?b.Holds(phi,a,b) & Holds(psi,b,a) & 
+ !b0.Holds(phi,a,b0) & Holds(psi,b0,a) ==> b0 = b’ >-- 
+ (rpt strip_tac >> first_x_assum (qspecl_then [‘a’,‘a’] assume_tac) >>
+  fs[] >> qexists_tac ‘b'’ >> arw[] >>
+  rpt strip_tac >> 
+  first_x_assum (qspecl_then [‘b0’,‘b'’] (assume_tac o GSYM)) >>
+  arw[] >> qexists_tac ‘a’ >> arw[]) >>
+ qby_tac ‘!b. ?a.Holds(phi,a,b) & Holds(psi,b,a) & 
+ !a0.Holds(phi,a0,b) & Holds(psi,b,a0) ==> a0 = a’ >--
+ (rpt strip_tac >> first_x_assum (qspecl_then [‘b’,‘b’] assume_tac) >>
+  fs[] >> qexists_tac ‘b'’ >> arw[] >>
+  rpt strip_tac >> 
+  first_x_assum (qspecl_then [‘a0’,‘b'’] (assume_tac o GSYM)) >>
+  arw[] >> qexists_tac ‘b’ >> arw[]) >>
+
+*)
+
+
+(*TODO: see why the gen var of a is b', not a'*)
 val Thm_2_7_bij = proved_th $
 e0
-(cheat)
+(rpt strip_tac >> rw[Bij_R_expand,id_def,R_EXT] >> dimp_tac >> strip_tac
+  (* 2 *)
+ >-- (qexists_tac ‘op(phi)’ >> rw[op_def,GSYM o_def] >> rpt strip_tac 
+      (* 2 *)
+      >-- (dimp_tac >> strip_tac (* 2 *)
+           >-- (first_x_assum irule >> qexists_tac ‘b'’ >> arw[]) >>
+           arw[] >> last_x_assum (qspecl_then [‘b’] strip_assume_tac) >>
+           qexists_tac ‘b'’ >> arw[]) >>
+      dimp_tac >> strip_tac (* 2 *)
+      >-- (first_x_assum irule >> qexists_tac ‘b'’ >> arw[]) >>
+      arw[] >> first_x_assum (qspecl_then [‘b’] strip_assume_tac) >>
+      qexists_tac ‘a'’ >> arw[]) >>
+ fs[GSYM o_def] >>
+ qby_tac ‘!a b. Holds(phi,a,b) <=> Holds(psi,b,a)’ >--
+ (rpt strip_tac >> dimp_tac >> strip_tac (* 2 *)
+  >-- (first_x_assum (qspecl_then [‘a’,‘a’] assume_tac) >> fs[] >>
+      qsuff_tac ‘b = b'’ >-- (strip_tac >> arw[]) >>
+      first_x_assum (qspecl_then [‘b'’,‘b’] (assume_tac o GSYM)) >>
+      fconv_tac (rewr_fconv (eq_sym "mem")) >> arw[] >>
+      qexists_tac ‘a’ >> arw[]) >>
+  first_x_assum (qspecl_then [‘b’,‘b’] assume_tac) >> fs[] >>
+  qsuff_tac ‘a = b'’ >-- (strip_tac >> arw[]) >>
+  first_x_assum (qspecl_then [‘b'’,‘a’] (assume_tac o GSYM)) >>
+  fconv_tac (rewr_fconv (eq_sym "mem")) >> arw[] >>
+  qexists_tac ‘b’ >> arw[])
+ >> rpt strip_tac (* 4 *)
+ >-- (first_x_assum (qspecl_then [‘a’,‘a’] assume_tac) >> fs[] >>
+     qexists_tac ‘b'’ >> arw[])
+ >-- (fs[] >> rev_full_simp_tac[] >> 
+     first_x_assum (qspecl_then [‘b1’,‘b2’] (assume_tac o GSYM)) >> 
+     arw[] >> qexists_tac ‘a’ >> arw[]) 
+ >-- (fs[] >> rev_full_simp_tac[] >> 
+     first_x_assum (qspecl_then [‘a1’,‘a2’] (assume_tac o GSYM)) >> 
+     arw[] >> qexists_tac ‘b’ >> arw[])
+ >-- (first_x_assum (qspecl_then [‘b’,‘b’] assume_tac) >> fs[] >>
+     qexists_tac ‘b'’ >> arw[])
+ )
 (form_goal
  “!A B phi:A->B.isBij(phi) <=> ?psi:B->A. psi o phi = id(A) & phi o psi = id(B)”)
 
@@ -427,19 +812,32 @@ For sets A and B, let ⊤:A↬B denote the relation such that ⊤(x,y) holds alw
 Theorem 2.8. For any sets A and B, A×B is a product of A and B in the category Set, and a coproduct in the category Rel.
 *)
 
+local 
+val lemma = fVar_Inst [("P",([("a",mem_sort (mk_set "A")),("b",mem_sort (mk_set "B"))],“T”))] (AX1 |> qspecl [‘A’,‘B’])
+in
+val T_uex = dimp_mp_l2r lemma (uex_def $ concl lemma) |> rewr_rule []
+                        |> gen_all
+end
+
 val T_ex = proved_th $
 e0
-cheat
+(assume_tac T_uex >> 
+ rpt strip_tac >> 
+ first_x_assum (qspecl_then [‘A’,‘B’] strip_assume_tac) >>
+ qexists_tac ‘R’ >> arw[] >> rpt strip_tac >> rw[])
 (form_goal
 “!A B. ?T0:A->B. !a b. Holds(T0,a,b)”)
 
 val Cross_ex = proved_th $
 e0
-(cheat)
+(rpt strip_tac >> 
+ qspecl_then [‘A’,‘B’] strip_assume_tac T_ex >>
+ qspecl_then [‘A’,‘B’,‘T0’] strip_assume_tac AX2 >> 
+ qexistsl_tac [‘TR’,‘p’,‘q’] >> fs[] >> rpt strip_tac >> rw[])
 (form_goal
- “!A B. ?AxB pi1:AxB ->A pi2:AxB ->B.
+ “!A B. ?AxB pi1:AxB ->A pi2:AxB ->B.isFun(pi1) & isFun(pi2) &
   (!x:mem(A) y:mem(B). ?r:mem(AxB).Eval(pi1,r) = x & Eval(pi2,r) = y) &
-   !r s. Eval(pi1,r) = Eval(pi1,s) & Eval(pi2,r) = Eval(pi2,s)
+   !r s. Eval(pi1,r) = Eval(pi1,s) & Eval(pi2,r) = Eval(pi2,s) ==> r = s
   ”)
 
 
@@ -461,38 +859,149 @@ val pi2_def =
 val _ = new_fun "Top" (rel_sort (mk_set "A") (mk_set "B"),
                        [("A",set_sort),("B",set_sort)])
 
-val _ = new_pred "isSetPr" [("p1",rel_sort (mk_set "AxB") (mk_set "A")),
+val _ = new_pred "SetPr" [("p1",rel_sort (mk_set "AxB") (mk_set "A")),
                             ("p2",rel_sort (mk_set "AxB") (mk_set "B"))]
 
 val SetPr_def = new_ax
 “!A B AxB p1:AxB->A p2:AxB->B. 
-isSetPr(p1,p2) <=>
-!X f:X->A g:X->B.isFun(f) & isFun(g) ==> ?!fg: X->AxB.p1 o fg = f & p2 o fg = g”
+ SetPr(p1,p2) <=>
+ !X f:X->A g:X->B.isFun(f) & isFun(g) ==> ?!fg: X->AxB.isFun(fg) & p1 o fg = f & p2 o fg = g”
 
 
 
-val _ = new_pred "isRelcP" [("i1",rel_sort (mk_set "A") (mk_set "AuB")),
+val _ = new_pred "RelcP" [("i1",rel_sort (mk_set "A") (mk_set "AuB")),
                             ("i2",rel_sort (mk_set "B") (mk_set "AuB"))]
 
 val RelcoPr_def = new_ax
 “!A B AuB i1:A->AuB i2:B->AuB. 
-isRelcP(i1,i2) <=>
+RelcP(i1,i2) <=>
 !X f:A->X g:B->X.?!fg:AuB ->X. fg o i1 = f & fg o i2 = g”
+
+(*
+
+TODO
+val uex_define_Fun = proved_th $
+e0
+()
+(form_goal “!a. ?!b.P(a,b) ==> ?!f:A->B.isFun(f) & !a. P(a,Eval(f,a))”)
+
+*)
+
+fun Cross A B = mk_fun "*" [A,B]
+
+val pi12_Fun = proved_th $
+e0
+(strip_tac >> strip_tac >>
+ qspecl_then [‘A’,‘B’] strip_assume_tac pi2_def >>
+ arw[])
+(form_goal
+“!A B. isFun(pi1(A,B)) & isFun(pi2(A,B))”)
+
+
+val Thm_2_7_o_Fun = proved_th $
+e0
+(rpt strip_tac >> fs[Fun_expand,GSYM o_def] >> rpt strip_tac (* 2 *)
+ >-- (last_x_assum (qspecl_then [‘a’] strip_assume_tac) >>
+      last_x_assum (qspecl_then [‘b’] strip_assume_tac) >>
+      qexistsl_tac [‘b'’,‘b’] >> arw[]) >>
+ first_x_assum irule >> 
+ qby_tac ‘b' = b’ >--
+ (first_x_assum irule >> qexistsl_tac [‘a’] >> arw[]) >>
+ fs[] >> qexists_tac ‘b’ >> arw[])
+(form_goal
+ “!A B f:A->B C g:B->C. isFun(f) & isFun(g) ==> isFun(g o f)”)
+
+val Holds_Eval = proved_th $
+e0
+(rpt strip_tac >> drule Eval_def >>
+ first_x_assum (qspecl_then [‘a’,‘Eval(f,a)’] assume_tac) >> fs[])
+(form_goal
+“!A B f:A->B. isFun(f) ==> !a.Holds(f,a,Eval(f,a))”)
+
+val o_Eval = proved_th $
+e0
+(rpt strip_tac >> 
+ qby_tac ‘isFun(g o f)’ >-- (irule Thm_2_7_o_Fun >> arw[]) >> 
+ drule $ GSYM Eval_def >> arw[] >>
+ rw[GSYM o_def] >> qexists_tac ‘Eval(f,a)’ >>
+ rev_drule $ GSYM Eval_def >>
+ first_x_assum (qspecl_then [‘a’,‘Eval(f,a)’] assume_tac) >> fs[] >>
+ qpick_x_assum ‘isFun(g)’ assume_tac >>
+ drule Holds_Eval >> arw[])
+(form_goal
+ “!A B f:A->B C g:B->C a:mem(A). isFun(f) & isFun(g) ==> 
+  Eval(g,Eval(f,a)) = Eval(g o f,a)”)
+
 
 val Thm_2_8_SetPr = proved_th $
 e0
-(cheat)
+(rpt strip_tac >> rw[SetPr_def] >> rpt strip_tac >>
+ rw[uex_def “?!fg:X-> A * B.isFun(fg) & pi1(A,B) o fg = f & pi2(A,B) o fg = g”] >>
+ strip_assume_tac $
+ uex_expand $ 
+ fVar_Inst 
+ [("P",([("x",mem_sort (mk_set "X")),
+        ("ab",mem_sort (Cross (mk_set"A") (mk_set "B")))],
+  “Eval(pi1(A,B),ab) = Eval(f:X->A,x) & 
+   Eval(pi2(A,B),ab) = Eval(g:X->B,x)”))] (AX1 |> qspecl [‘X’,‘A * B’]) >>
+ qexists_tac ‘R’ >> 
+ qspecl_then [‘A’,‘B’] strip_assume_tac pi2_def >>
+ qby_tac ‘isFun(R)’ >--
+ (arw[Fun_expand] >> 
+  rpt strip_tac (* 2 *) >-- 
+  (first_x_assum (qspecl_then [‘Eval(f,a)’,‘Eval(g,a)’] assume_tac) >>
+   arw[]) >>
+  first_x_assum irule >> arw[]) >> arw[] >>
+ qby_tac ‘pi1(A, B) o R = f & pi2(A, B) o R = g’ >--
+ (arw[R_EXT,GSYM o_def] >> rpt strip_tac (* 2 *) 
+  >-- (assume_tac Eval_def >> 
+       first_assum (qspecl_then [‘A * B’,‘A’,‘pi1(A,B)’] assume_tac) >>
+       first_x_assum drule >>
+       first_x_assum (qspecl_then [‘X’,‘A’,‘f’] assume_tac) >>
+       first_x_assum drule >> arw[] >>
+       dimp_tac >> strip_tac (* 2 *) >-- arw[] >>
+       first_x_assum 
+        (qspecl_then [‘Eval(f,a)’,‘Eval(g,a)’] strip_assume_tac) >>
+       qexists_tac ‘r’ >> arw[]) >>
+ assume_tac Eval_def >> 
+ first_assum (qspecl_then [‘A * B’,‘B’,‘pi2(A,B)’] assume_tac) >>
+ first_x_assum drule >>
+ first_x_assum (qspecl_then [‘X’,‘B’,‘g’] assume_tac) >>
+ first_x_assum drule >> arw[] >>
+ dimp_tac >> strip_tac (* 2 *) >-- arw[] >>
+ first_x_assum 
+  (qspecl_then [‘Eval(f,a)’,‘Eval(g,a)’] strip_assume_tac) >>
+ qexists_tac ‘r’ >> arw[]) >> arw[] 
+ (*last subgoal*)
+ >>
+ rpt strip_tac >> first_x_assum irule >> 
+ drule Eval_def >> arw[] >> pop_assum (K all_tac) >>
+ rpt strip_tac >> dimp_tac >> strip_tac (* 2 *)
+ >-- (once_arw[] >>
+     qby_tac ‘Eval(pi1(A, B), Eval(fg', a)) = Eval(pi1(A,B) o fg',a) & 
+              Eval(pi2(A, B), Eval(fg', a)) = Eval(pi2(A,B) o fg',a)’
+     >-- (strip_tac >> irule o_Eval >> arw[]) >>
+     arw[]) >>
+ first_x_assum irule >> arw[] >> strip_tac >> 
+ fconv_tac (rewr_fconv (eq_sym "mem")) (* 2 *)
+ >-- (qpick_x_assum ‘pi2(A, B) o fg' = g’ (assume_tac o GSYM) >>
+      once_arw[] >> irule o_Eval >> arw[]) >>
+ qpick_x_assum ‘pi1(A, B) o fg' = f’ (assume_tac o GSYM) >>
+ once_arw[] >> irule o_Eval >> arw[]
+ )
 (form_goal
-“!A B. isSetPr(pi1(A,B),pi2(A,B))”)
+“!A B. SetPr(pi1(A,B),pi2(A,B))”)
+
 
 val SPa_ex =
 let val th0 = rewr_rule[SetPr_def] Thm_2_8_SetPr
     val f = th0 |> spec_all |> concl |> snd o dest_imp
-    val th1 = uex_ex f
+    val th1 = uex_def f
     val th0' = strip_all_and_imp th0
-    val th2 = mp th1 th0' 
+    val th2 = dimp_mp_l2r th0' th1 
 in disch_all th2 |> gen_all
 end 
+
 
 (*
 
@@ -564,24 +1073,115 @@ val SetEz_def = new_ax
 “!A B f:A->B g:A->B E e:E->A. SetEz(f,g,e) <=>
  isFun(f) & isFun(g) & isFun(e) & !X x:X->A.isFun(x) & f o x = g o x ==> ?!x0:X->E. isFun(x0) & x = e o x0”
 
+(*
+fVar_Inst [("P",([("a",mem_sort (mk_set "A"))],“Eval(f:A->B,a) = Eval(g:A->B,a)”))] (Thm_2_4 |> qspecl [‘A’])
+example of current fvar doing ill-=formed form, f and g
+
+
+*)
+val Inj_Fun = proved_th $
+e0
+(rw[Inj_def] >> rpt strip_tac >> arw[])
+(form_goal
+ “!A B f:A->B. isInj(f) ==> isFun(f)”)
+
+val Inj_lcancel = proved_th $
+e0
+(rpt strip_tac >> fs[Inj_def] >>
+ irule $ iffRL FUN_EXT >> arw[] >> strip_tac >> 
+ qsuff_tac ‘Eval(m,Eval(f,a)) = Eval(m,Eval(g,a))’ >--
+ (strip_tac >> first_x_assum irule >> arw[]) >>
+ qby_tac ‘Eval(m, Eval(f, a)) = Eval(m o f,a) &
+          Eval(m, Eval(g, a)) = Eval(m o g,a)’
+ >-- (strip_tac >> irule o_Eval >> arw[]) >>
+ arw[])
+(form_goal
+ “!A B m:A->B.isInj(m) ==>
+  !X f:X->A g:X->A. isFun(f) & isFun(g) & m o f = m o g ==> f = g”)
+
+local
+val lemma =
+fVar_Inst [("P",([("a",mem_sort (mk_set "A"))],“Eval(f:A->X,a) = Eval(g:A->X,a)”))] (Thm_2_4|> qspecl [‘A’]) |> gen_all
+val lemma1 = 
+fVar_Inst [("P",([("a0",mem_sort (mk_set "X")),("a0'",mem_sort (mk_set "E"))],“Eval(e:E->A,a0') = Eval(x:X->A,a0)”))] (AX1|> qspecl [‘X’,‘E’])
+|> uex_expand
+in
 val Thm_2_9_Eqlz = proved_th $
 e0
-(cheat)
+(rpt strip_tac >> rw[SetEz_def] >>
+ qspecl_then [‘A’,‘B’,‘f’,‘g’]
+  (x_choosel_then ["E","e"] strip_assume_tac) lemma >>
+ qexistsl_tac [‘E’,‘e’] >> arw[] >> 
+ drule Inj_Fun >> arw[] >> rpt strip_tac >>
+ rw[uex_def “?!x0:X->E. isFun(x0) & x = e o x0”] >>
+ strip_assume_tac lemma1 >>
+ qexists_tac ‘R’ >> 
+ qby_tac ‘isFun(R)’ >--
+ (arw[Fun_expand] >> rpt strip_tac >--
+  (fconv_tac (once_depth_fconv no_conv (rewr_fconv (eq_sym "mem"))) >>
+  last_x_assum $ assume_tac o iffLR >>
+  first_x_assum irule >> 
+  qsuff_tac ‘Eval(f,Eval(x,a)) = Eval(f o x,a) & 
+             Eval(g,Eval(x,a)) = Eval(g o x,a)’
+  >-- (strip_tac >> fs[]) >>
+  strip_tac (* 2 *) >> irule o_Eval >> arw[]) >>
+  fs[Inj_def] >> first_x_assum irule >> arw[]) >>
+ arw[] >> 
+ qby_tac ‘x = e o R’ >--
+ (drule Eval_def >> fs[] >>
+  qby_tac ‘isFun(e o R)’ >-- (irule Thm_2_7_o_Fun >> arw[]) >>
+  irule (iffRL FUN_EXT) >>
+  arw[] >> strip_tac >>
+  qby_tac ‘Eval(e o R,a) = Eval(e,Eval(R,a))’
+  >-- (irule $ GSYM o_Eval >> arw[]) >>
+  arw[] >> last_x_assum (qspecl_then [‘a’,‘Eval(R,a)’] assume_tac) >>
+  fs[]) >> arw[] >>
+ rpt strip_tac >> irule Inj_lcancel >> arw[] >>
+ qexistsl_tac [‘A’,‘e’] >> arw[])
 (form_goal
 “!A B f:A->B g:A->B.isFun(f) & isFun(g) ==> ?E e:E->A.SetEz(f,g,e)”)
+end
 
 (*
 
 Theorem 2.10. For any function f:A→B we have f=me, where m:im(f)↪B is an injection and e:A↠im(f) is a surjection. A set im(f) equipped with such m and e is unique up to bijection and is called the image of f.
 
+Proof. Let im(f) be |S| where S is defined by y∈S iff there exists an x∈A with f(x)=y. By definition, we have an injection m:im(f)↪B. And for any x∈A, clearly f(x)∈S, so there is a unique y∈im(f) with m(y)=f(x); we define e(x)=y. It is easy to verify the rest.  ▮
 
 *)
 
+local
+val lemma =
+fVar_Inst [("P",([("b",mem_sort (mk_set "B"))],“?a:mem(A).Eval(f:A->B,a) = b”))] (Thm_2_4|> qspecl [‘B’]) 
+val lemma1 = 
+fVar_Inst [("P",([("x",mem_sort (mk_set "A")),("y",mem_sort (mk_set "s"))],“Eval(f:A->B,x) = Eval(m:s->B,y)”))] (AX1|> qspecl [‘A’,‘s’]) |> uex_expand
+in
 val Thm_2_10 = proved_th $
 e0
-(cheat)
+(rpt strip_tac >> 
+ x_choosel_then ["s","m"] strip_assume_tac lemma >>
+ x_choose_then "e" strip_assume_tac lemma1 >>
+ qexistsl_tac [‘s’,‘e’,‘m’] >> 
+ arw[] >>
+ qby_tac ‘isFun(e)’ >--
+ (rw[Fun_expand] >> arw[] >> rpt strip_tac (* 2 *)
+  >-- (last_x_assum $ irule o iffLR >> qexists_tac ‘a’ >> rw[]) >>
+  fs[Inj_def] >> first_x_assum irule >> arw[]) >>
+ qby_tac ‘isSurj(e)’ >--
+ (arw[Surj_def] >> strip_tac >> drule Eval_def >> fs[] >> 
+  fconv_tac (once_depth_fconv no_conv (rewr_fconv (eq_sym "mem"))) >>
+  arw[] >> qexists_tac ‘y’ >> rw[]) >> arw[] >>
+ qby_tac ‘isFun(m o e)’ >-- (irule Thm_2_7_o_Fun >> arw[] >>
+ fs[Inj_def]) >>
+ irule $ iffRL FUN_EXT >> arw[] >> strip_tac >>
+ qpick_x_assum ‘isFun(e)’ assume_tac >> drule Eval_def >> fs[] >>
+ last_x_assum (qspecl_then [‘a’,‘Eval(e,a)’] assume_tac) >> fs[] >>
+ irule o_Eval >> arw[] >> fs[Inj_def])
 (form_goal
-“!A B f:A->B. isFun(f) ==> ?M e:A->M m:M->B. f = m o e & isInj(e) & isSurj(m)”)
+“!A B f:A->B. isFun(f) ==> ?M e:A->M m:M->B. f = m o e & isSurj(e) & isInj(m)”)
+end
+
+(*TODO: 2.10 unique upto bijection*)
 
 
 (*2.11 left to tomorrow...*)
@@ -593,7 +1193,7 @@ Axiom 3 (power sets): For any set A, there exists a set PA and a relation ϵ:A�
 (*val _ = new_fun "Pow" (set_sort,[("A",set_sort)]) *)
 
 val AX3 = new_ax 
-“!A. ?PA e:A->PA. !S0:1->A.?!s:mem(PA). !x:mem(A). Holds(S0,star,x) <=> 
+“!A. ?PA e:A->PA. !S0:1->A.?!s:mem(PA). !x:mem(A). Holds(S0,dot,x) <=> 
  Holds(e,x,s)”
 
 (*
@@ -606,9 +1206,9 @@ val Pow_def =
         |> C mp (trueI []) |> gen_all
 
 
-val eps_def = 
+val In_def = 
     Pow_def |> spec_all |> eqT_intro 
-            |> iffRL |> ex2fsym "eps" ["A"] 
+            |> iffRL |> ex2fsym "In" ["A"] 
             |> C mp (trueI []) |> gen_all
 
 
@@ -794,28 +1394,161 @@ cheat
  “!A B r:A->B C s:A->C. ?sdr:B->C. 
   !t.Sub(t,sdr) <=> Sub(t o r,s)”)
 
+(*
+Theorem 2.12. For any relation R:B↬A, there exists a unique function fR:B→PA such that R(y,x) if and only if ϵ(x,fR(y)). It follows that Set is a topos (and Rel is a power allegory).
+Proof. We simply define fR elementwise; for each y we define fR(y) to be the unique element of PA such that ϵ(x,fR(y)) holds iff R(y,x) holds. Extensionality of functions implies that it is unique.  ▮
+*)
+fun Pow A = mk_fun "Pow" [A]
+
+val uex_tac:tactic = fn (ct,asl,w) =>
+    let val th = uex_def w
+        val w' = snd $ dest_dimp $ concl th
+    in ([(ct,asl,w')],(sing (dimp_mp_r2l th)))
+    end
+
+
+local 
+val lemma = 
+fVar_Inst 
+[("P",([("star",mem_sort ONE),("a",mem_sort (mk_set "A"))],
+“(?a0. a = Eval(s0:A0->A,a0))”))]
+(AX1|> qspecl [‘1’,‘A’]) 
+|> uex_expand 
+in
+(*todo: both once_depth_fconv and basic_once_fconv cannot turn the a into dot*)
+val In_def_Inj = proved_th $
+e0
+(rpt strip_tac >> assume_tac In_def >>
+ strip_assume_tac lemma >>
+ first_x_assum (qspecl_then [‘A’,‘R’] $ strip_assume_tac o uex_expand) >>
+ uex_tac >>
+ qexists_tac ‘s’ >> 
+ qpick_x_assum ‘!a b. Holds(R,a,b) <=> ?a0.b = Eval(s0,a0)’
+ (mp_tac o GSYM) >> once_rw[dot_def] >> strip_tac >>
+ first_x_assum (qspecl_then [‘dot’] assume_tac) >> arw[] >>
+ rev_full_simp_tac[] >> rpt strip_tac >> rw[]
+ )
+(form_goal
+“!A A0 s0:A0->A.isInj(s0) ==>
+ ?!s:mem(Pow(A)).!x:mem(A). (?a0.x = Eval(s0,a0)) <=> Holds(In(A),x,s)”)
+end
+
+(*In_def_P currently have to be like this because if there is P(a)in the assumption then every arw causes mess, extremely ugly, need to fix this*)
+local
+val lemma = 
+fVar_Inst 
+[("P",([("a",mem_sort (mk_set "A"))],
+“(?a0. a = Eval(s0:A0->A,a0))”))]
+(Thm_2_4 |> qspecl [‘A’]) 
+in
+val In_def_P = proved_th $
+e0
+(strip_tac >> uex_tac >> 
+ strip_assume_tac $ spec_all Thm_2_4 >>
+ drule In_def_Inj >> pop_assum (strip_assume_tac o uex_expand) >>
+ qexists_tac ‘s’ >> strip_tac (* 2 *)>--
+ (strip_tac >> 
+ first_x_assum (qspecl_then [‘a’] assume_tac) >>
+ first_x_assum (qspecl_then [‘a’] assume_tac) >>
+ accept_tac
+ (iff_trans (assume “P(a:mem(A)) <=> ?b:mem(B).a = Eval(i:B->A,b)”)
+            (assume “(?a0.a = Eval(i:B->A,a0)) <=> Holds(In(A),a,s)”))) >>
+ rpt strip_tac >> first_x_assum irule >>
+ strip_tac >>
+ first_x_assum (qspecl_then [‘x’] assume_tac) >>
+ last_x_assum (qspecl_then [‘x’] assume_tac) >>
+ accept_tac
+ (iff_trans 
+  (GSYM $ assume “P(x) <=> ?b.x = Eval(i:B->A,b)”)
+  (assume “P(x:mem(A)) <=> Holds(In(A),x,s')”)))
+(form_goal
+ “!A.?!s:mem(Pow(A)).!a.P(a) <=> Holds(In(A),a,s)”)
+end
+
+local
+val lemma = 
+fVar_Inst 
+[("P",([("a",mem_sort (mk_set "A"))],
+“Holds(In(A),a,s1)”))]
+(In_def_P|> qspecl [‘A’]) |> uex_expand
+in
+val In_EXT = proved_th $
+e0
+(rpt strip_tac >> strip_assume_tac lemma >>
+ qsuff_tac ‘s1 = s & s2 = s’ >-- (strip_tac >> arw[]) >>
+ strip_tac >> first_x_assum irule >> rpt strip_tac (*2  *)
+ >-- rw[] >> pop_assum (K all_tac) >> arw[])
+(form_goal
+ “!A s1:mem(Pow(A)) s2. (!x.Holds(In(A),x,s1) <=> Holds(In(A),x,s2)) ==>
+ s1 = s2”)
+end
+
+local
+val lemma = 
+fVar_Inst 
+[("P",([("y",mem_sort (mk_set "B")),("s",mem_sort (Pow (mk_set "A")))],
+“!x.Holds(In(A),x,s) <=> Holds(R:B->A,y,x)”))]
+(AX1|> qspecl [‘B’,‘Pow(A)’]) |> uex_expand
+val lemma1 = 
+fVar_Inst 
+[("P",([("x",mem_sort (mk_set "A"))],
+“Holds(R:B->A,a,x)”))]
+(In_def_P|> qspecl [‘A’]) |> uex_expand
+in
 val Thm_2_12 = proved_th $
 e0
-(cheat)
+(rpt strip_tac >>
+ x_choose_then "fR" strip_assume_tac lemma >>
+ uex_tac >> qexists_tac ‘fR’ >>
+ qby_tac ‘isFun(fR)’ >-- 
+ (arw[Fun_expand] >> rpt strip_tac (* 2 *) >--
+  (strip_assume_tac lemma1 >> qexists_tac ‘s’ >> arw[] >>
+   strip_tac >> rw[]) >>
+  strip_assume_tac lemma1 >> 
+  qsuff_tac ‘b1 = s & b2 = s’ >-- (strip_tac >> arw[]) >>
+  strip_tac >> first_x_assum irule >> arw[] >> strip_tac >> rw[]) >>
+ arw[] >>
+ qby_tac
+ ‘!y x.Holds(R,y,x) <=> Holds(In(A),x,Eval(fR,y))’ >--
+ (drule Eval_def >> fs[] >> rpt strip_tac >>
+ last_x_assum (qspecl_then [‘y’,‘Eval(fR,y)’] assume_tac) >>
+ fs[]) >> arw[] >> (* TODO, should not need strip_tac, should directly have one conj remaining*) rpt strip_tac >> rw[] >>
+ first_x_assum irule >> rpt strip_tac >>
+ drule Eval_def >> arw[] >> dimp_tac >> rpt strip_tac (* 2 *)
+ >-- arw[] >> irule In_EXT >> arw[] >> rpt strip_tac >> rw[])
 (form_goal
-“!B A R:B->A.?!fR:B->Pow(A).isFun(fR) & !y x.(Holds(R,y,x) <=> Holds(eps(A),x,Eval(fR,y)))”)
-
-(*
-Theorem 2.13. For any two sets A and B, there exists a set BA and a function ev:BA×A→B such that for any function f:A→B there exists a unique element sf∈BA such that ev(sf,a)=f(a) for all a∈A. It follows that Set is a cartesian closed category.
-*)
+“!B A R:B->A.?!fR:B->Pow(A).isFun(fR) & !y x.(Holds(R,y,x) <=> Holds(In(A),x,Eval(fR,y)))”)
+end
 
 
-val Thm_2_3_5 = proved_th $
+local
+val lemma =
+(fVar_Inst [("P",([("star",mem_sort ONE),("x",mem_sort (mk_set "A"))],“x = a:mem(A)”))] (AX1 |> qspecl [‘1’,‘A’])) |> uex_expand
+in
+val Thm_2_3_5_el = proved_th $
 e0
-cheat
+(rpt strip_tac >> uex_tac >>
+ strip_assume_tac lemma >> qexists_tac ‘R’ >>
+ qby_tac ‘isFun(R)’ >--
+ (arw[Fun_expand] >> once_rw[dot_def] >> rpt strip_tac (* 2 *)
+ >-- (qexists_tac ‘a’ >> rw[]) >-- arw[]) >>
+ arw[] >>
+ qby_tac ‘Eval(R,dot) = a’ >--
+ (drule Eval_def >> fs[] >>
+  last_x_assum (qspecl_then [‘dot’,‘a’] assume_tac) >> fs[]) >>
+ arw[] >>
+ rpt strip_tac >> first_x_assum irule >>
+ rpt strip_tac >> once_rw[dot_def] >> 
+ drule Eval_def >> fs[])
 (form_goal
- “!A a:mem(A). ?!R:1->A. isFun(R) & Eval(R,star) = a”)
+ “!A a:mem(A). ?!R:1->A. isFun(R) & Eval(R,dot) = a”)
+end
 
 (*mem as fun*)
 val MF_def =
-let val f = concl $ spec_all Thm_2_3_5
+let val f = concl $ spec_all Thm_2_3_5_el
     val uth = uex_def f
-    val th = dimp_mp_l2r (spec_all Thm_2_3_5) uth
+    val th = dimp_mp_l2r (spec_all Thm_2_3_5_el) uth
 in
 th |> eqT_intro |> iffRL |> ex2fsym "MF"["a"]
    |> C mp (trueI []) |> gen_all
@@ -829,12 +1562,16 @@ e0
 “!A B a:mem(A) b:mem(B).Eval(Spa(MF(a),MF(b)),star)”)
 *)
 
+(*
+Theorem 2.13. For any two sets A and B, there exists a set BA and a function ev:BA×A→B such that for any function f:A→B there exists a unique element sf∈BA such that ev(sf,a)=f(a) for all a∈A. It follows that Set is a cartesian closed category.
+*)
+
 val Thm_2_13 = proved_th $
 e0
 (cheat)
 (form_goal
 “!A B.?A2B ev:A2B * A ->B. isFun(ev) & 
- !f:A->B.isFun(f) ==> ?!sf:mem(A2B).!a:mem(A).Eval(ev,Eval(SPa(MF(sf),MF(a)),star)) = Eval(f,a)”)
+ !f:A->B.isFun(f) ==> ?!sf:mem(A2B).!a:mem(A).Eval(ev,Eval(SPa(MF(sf),MF(a)),dot)) = Eval(f,a)”)
 
 (*
 
@@ -1014,20 +1751,6 @@ In which case will we need / should we allow partial application
 
 (* (P(a) ==> P(f(a))) ===> ...*)
 
-fun fVar_Inst (pair as (P,(argl:(string * sort) list,Q))) f = 
-    case view_form f of
-        vfVar(P0,args0) =>
-(*ListPair.map ListPair.foldl*)
-(*mk_inst (zip argl args0)ListPair. [] *)
-        if P0 = P then
-            let val venv = match_tl essps (List.map mk_var argl) args0 emptyvd 
-            in inst_form (mk_menv venv emptyfvd) Q
-            end
-(*if the number of arguments is wrong, or the sorts is wrong, then handle the matching exn by returning f *)
-        else f
-      | vConn(co,fl) => mk_conn co (List.map (fVar_Inst pair) fl)
-      | vQ(q,n,s,b) => mk_quant q n s (fVar_Inst pair b)
-      | vPred _ => f
 
 P(a:mem(A),b:mem(B))
 
